%%%%%%%%%%%%%%%%%%%%%%%%%%%%%%%%%%%%%%%%%%%%%%%%%%%%%%%%%%%%%%%%%%%%%%%%%%%%%%%%%
\clearpage
Example: 已知$abc=1$, 求$\frac{a}{ab+a+1}+\frac{b}{bc+c+1}+\frac{c}{ca+c+1}$  
\clearpage
Hints:
\begin{itemize}
\item 将某个$1$替换成$abc$试着计算看看
\end{itemize}

%%%%%%%%%%%%%%%%%%%%%%%%%%%%%%%%%%%%%%%%%%%%%%%%%%%%%%%%%%%%%%%%%%%%%%%%%%%%%%%%%
\clearpage
将上面的情形推广到$abcd=1$


%%%%%%%%%%%%%%%%%%%%%%%%%%%%%%%%%%%%%%%%%%%%%%%%%%%%%%%%%%%%%%%%%%%%%%%%%%%%%%%%%
\clearpage
Example: 已知$a+b+c=abc$, 求证$a(1-b^2)(1-c^2)+b(1-a^2)(1-c^2)+c(1-a^2)(1-b^2)
         =4abc$  
\clearpage
Hints:
\begin{itemize}
\item a+b=abc-c
\item 三角函数背景
\end{itemize}


%%%%%%%%%%%%%%%%%%%%%%%%%%%%%%%%%%%%%%%%%%%%%%%%%%%%%%%%%%%%%%%%%%%%%%%%%%%%%%%%%
\clearpage
Example: 证明 $((a-b)^2+(b-c)^2+(c-a)^2)^2=2((a-b)^4+(b-c)^4+(c-a)^4)$
\clearpage
Hints:
\begin{itemize}
\item if $a+b+c=0$, $(a^2+b^2+c^2)^2=2(a^4+b^4+c^4)$
\end{itemize}


%%%%%%%%%%%%%%%%%%%%%%%%%%%%%%%%%%%%%%%%%%%%%%%%%%%%%%%%%%%%%%%%%%%%%%%%%%%%%%%%%
\clearpage
Example: $a+b+c=0$, 证明:
$2(a^5+b^5+c^5)=5abc(a^2+b^2+c^2)$,
$5(a^3+b^3+c^3)(a^2+b^2+c^2)=6(a^5+b^5+c^5)$,
$10(a^7+b^7+c^7)=7(a^2+b^2+c^2)(a^5+b^5+c^5)$
\clearpage
Hints:
\begin{itemize}
\item 
\end{itemize}


%%%%%%%%%%%%%%%%%%%%%%%%%%%%%%%%%%%%%%%%%%%%%%%%%%%%%%%%%%%%%%%%%%%%%%%%%%%%%%%%%
\clearpage
Example: Given $(1+\sin A)(1+\sin B)(1+\sin C)=\cos A\cos B\cos C$,
simplify $(1-\sin A)(1-\sin B)(1-\sin C)$ 
\clearpage
Hints:
\begin{itemize}
\item 
\end{itemize}

















































