%%%%%%%%%%%%%%%%%%%%%%%%%%%%%%%%%%%%%%%%%%%%%%%%%%%%%%%%%%%%%%%%%%%%%%%%%%%%%%%5
\clearpage
Example: $xyz\geq 1$, prove $\sum \frac{x^5-x^2}{x^5+y^2+z^2}\geq 0$ 
\clearpage
Hints:
\begin{itemize}
\item $deg(x^5)-deg(x^2,y^2,z^2)=deg(xyz)$ 
\end{itemize}


%%%%%%%%%%%%%%%%%%%%%%%%%%%%%%%%%%%%%%%%%%%%%%%%%%%%%%%%%%%%%%%%%%%%%%%%%%%%%%%5
\clearpage
Example: Consider the expression:
$S=f(a,b,c)=S_a(b-c)^2+S_b(a-c)^2+S_c(a-b)^2$, where $S_a, S_b, S_c$ are functions
of $a,b,c$:
\begin{itemize}
\item if $S_a,S_b,S_c\geq 0$, then $S\geq 0$
\item if $a\geq b\geq c$ and $S_b, S_b+S_a, S_b+S_c\geq 0$, then $S\geq 0$
\item if $a\geq b\geq c$ and $S_a, S_c, S_a+2S_b, S_c+2S_b\geq 0$, then $S\geq 0$
\item if $a\geq b\geq c$ and $S_a, S_c, a^2S_b+b^2S_a\geq 0$, then $S\geq 0$
\item if $a\geq b\geq c$ and $(a-c)S_b+(a-b)S_c, (a-c)S_b+(b-c)S_a\geq 0$, then $S\geq 0$
\item if $a\geq b\geq c$ and $S_b, S_c, (a-c)S_b+(b-c)S_a\geq 0$, then $S\geq 0$ 
\item if $S_a+S_b+S_c\geq 0$ and $S_aS_b+S_aS_c+S_bS_c\geq 0$, then $S\geq 0$
\end{itemize}
\clearpage
Hints:
\begin{itemize}
\item Given an expression, we can transform it to basic sos form, if it is sysmetric 
or ayclic function $f(a,b,c)$ satisfy $f(a,a,a)=0$ 
\end{itemize}


%%%%%%%%%%%%%%%%%%%%%%%%%%%%%%%%%%%%%%%%%%%%%%%%%%%%%%%%%%%%%%%%%%%%%%%%%%%%%%%5
\clearpage
Example: $a,b,c>0$, then $\frac{a^2+b^2+c^2}{ab+bc+ca}+\frac{8abc}{(a+b)(b+c)(c+a)}\geq 2$
 

%%%%%%%%%%%%%%%%%%%%%%%%%%%%%%%%%%%%%%%%%%%%%%%%%%%%%%%%%%%%%%%%%%%%%%%%%%%%%%%5
\clearpage
Example: $x,y,z>0$, then $\frac{1}{(x+y)^2}+\frac{1}{(y+z)^2}+\frac{1}{(x+z)^2}\geq
\frac{9}{4(xy+yz+xz)}$ 





















